reverted to putting module and its associated methods together

ComposableModules.v
@@ -6,26 +6,45 @@ From Stdlib Require Import Program.Equality.
 Set Implicit Arguments.
 Set Asymmetric Patterns.
 
+(** 1. Recursive Method Tuple Type Family *)
+Fixpoint Methods (sigs : list (Kind * Kind)) (t : Tree Elem) : Type :=
+  match sigs with
+  | [] => unit
+  | (K_in, K_out) :: sigs' => (type K_in -> Action type t K_out) ** Methods sigs' t
+  end.
+
+(** 2. Multi-Method Module Types *)
 Inductive ModuleType : Type :=
-| MkMod : ModuleType
-| MkMeth (K_in K_out : Kind) : ModuleType
+| MkMod (sigs : list (Kind * Kind)) : ModuleType
 | BindMod (B : ModuleType) : ModuleType
 | BindMeth (K_in K_out : Kind) (B : ModuleType) : ModuleType.
 
+(** 3. Denotational Semantics *)
 Fixpoint ModuleSem (mt : ModuleType) (t_acc : Tree Elem) (t_curr : Tree Elem) : Type :=
   match mt with
-  | MkMod => Mod (Node "" [t_acc; t_curr])
-  | MkMeth K_in K_out => type K_in -> Action type (Node "" [t_acc; t_curr]) K_out
+  | MkMod sigs => Mod (Node "" [t_acc; t_curr]) ** Methods sigs (Node "" [t_acc; t_curr])
   | BindMod B => forall (t_new : Tree Elem), Mod t_new -> ModuleSem B (Node "" [t_acc; t_curr]) t_new
   | BindMeth K_in K_out B => (type K_in -> Action type t_curr K_out) -> ModuleSem B t_acc t_curr
   end.
 
+(** 4. Method Simulation definitions *)
 Definition MethSimulation {t1 t2: Tree Elem} {K_in K_out: Kind}
   (M1: type K_in -> Action type t1 K_out) (M2: type K_in -> Action type t2 K_out)
   (rel: TreeState ElemState t1 -> TreeState ElemState t2 -> Prop) : Prop :=
   forall (v_in : type K_in),
     ActionSimulation (M1 v_in) (M2 v_in) rel.
 
+Fixpoint MethodsSimulation (sigs : list (Kind * Kind)) (t1 t2 : Tree Elem)
+  (rel : TreeState ElemState t1 -> TreeState ElemState t2 -> Prop) {struct sigs} :
+  Methods sigs t1 -> Methods sigs t2 -> Prop :=
+  match sigs with
+  | [] => fun _ _ => True
+  | (K_in, K_out) :: sigs' => fun meths1 meths2 =>
+      MethSimulation meths1.(Fst) meths2.(Fst) rel /\
+      MethodsSimulation sigs' t1 t2 rel meths1.(Snd) meths2.(Snd)
+  end.
+
+(** 5. Simulation Relation *)
 Fixpoint Simulation (mt : ModuleType)
                      (t_acc1 t_acc2 : Tree Elem)
                      (rel_acc : TreeState ElemState t_acc1 -> TreeState ElemState t_acc2 -> Prop)
@@ -33,10 +52,10 @@ Fixpoint Simulation (mt : ModuleType)
                      (rel_curr : TreeState ElemState t_curr1 -> TreeState ElemState t_curr2 -> Prop)
                      (m1 : ModuleSem mt t_acc1 t_curr1) (m2 : ModuleSem mt t_acc2 t_curr2) : Prop :=
   match mt as mt0 return ModuleSem mt0 t_acc1 t_curr1 -> ModuleSem mt0 t_acc2 t_curr2 -> Prop with
-  | MkMod => fun m1 m2 =>
-      ModSimulation m1 m2 (fun s1 s2 => rel_acc s1.(Fst) s2.(Fst) /\ rel_curr s1.(Snd).(Fst) s2.(Snd).(Fst))
-  | MkMeth K_in K_out => fun m1 m2 =>
-      MethSimulation m1 m2 (fun s1 s2 => rel_acc s1.(Fst) s2.(Fst) /\ rel_curr s1.(Snd).(Fst) s2.(Snd).(Fst))
+  | MkMod sigs => fun m1 m2 =>
+      let rel_comb := fun s1 s2 => rel_acc s1.(Fst) s2.(Fst) /\ rel_curr s1.(Snd).(Fst) s2.(Snd).(Fst) in
+      ModSimulation m1.(Fst) m2.(Fst) rel_comb /\
+      MethodsSimulation sigs (Node "" [t_acc1; t_curr1]) (Node "" [t_acc2; t_curr2]) rel_comb m1.(Snd) m2.(Snd)
   | BindMod B => fun F1 F2 =>
       forall (t_new1 t_new2 : Tree Elem)
              (m1_in : Mod t_new1)
